theories/unif.v
@@ -11,15 +11,21 @@ Section s.
 (* Notation unify := (unify u). *)
 Notation vars := vars_tm.
 
-Definition matching_var (s: Sigma) (query:V) (arg: Tm) := 
-  @None Sigma.
+Definition compare_var '(IV v1) '(IV v2) := 
+  if v1 <= v2 then (IV v1, IV v2) else (IV v2, IV v1).
 
-Definition unify_var (s:Sigma) v arg := 
+Definition unify_var (s:Sigma) (v:V) arg := 
   if v \in vars_tm arg then None
-  else Some s.[v <- arg].
+  else 
+    match arg with
+    | Tm_V v' =>
+      let: (v1, v2) := compare_var v v' in Some s.[v1 <- Tm_V v2]
+    | _ => Some s.[v <- arg]
+    end.
+    (* Some s.[v <- arg]. *)
 
-Fixpoint unifier_help var_matcher n query pat s :=
-  let unifier_help := unifier_help var_matcher in
+Fixpoint unifier_help is_matchin n query pat s :=
+  let unifier_help := unifier_help is_matchin in
   let query := deref s query in
   let pat := deref s pat in
   if query == pat then Some s
@@ -31,13 +37,13 @@ Fixpoint unifier_help var_matcher n query pat s :=
     | Tm_V v' => unify_var s v' query
     | Tm_D _ | Tm_P _ =>
         match query with 
-        | Tm_V v => var_matcher s v pat
+        | Tm_V v => if is_matchin then None else unify_var s v pat
         | _ => None
         end
     | Tm_App t1 t2 =>
       match query with
       | Tm_App tx ty => obind (unifier_help n ty t2) (unifier_help n tx t1 s)
-      | Tm_V v => var_matcher s v pat
+      | Tm_V v => if is_matchin then None else unify_var s v pat
       | _ => None
       end
     end
@@ -49,32 +55,48 @@ Fixpoint size_tm t :=
   | _ => 1
   end.
 
-Definition vars_nb t1 t2 := ((#|` vars_tm t1 |) + #|` vars_tm t2|)%nat.
+(* Definition vars_nb t1 t2 s := (size (vars_tmL t1) + size (vars_tmL t2) + #|` vars_sigma s|)%nat. *)
 
-Definition matching_aux := unifier_help matching_var.
-Definition matching t1 t2 s := matching_aux (vars_nb t1 t2) t1 t2 s.
+Definition unifier_help1 b t1 t2 s :=
+  omap (fun x => s + x) (unifier_help b (size_tm t1 + size_tm t2) t1 t2 s).
 
-Definition unify_aux := unifier_help unify_var.
-Definition unify t1 t2 s := unify_aux (vars_nb t1 t2) t1 t2 s.
+Definition unifier_help2 b t1 t2 s := unifier_help1 b (deref s t1) (deref s t2) s.
 
-Lemma unify_V_empty v t:
-  v \notin vars_tm t ->
-  unify (Tm_V v) t empty = if t is Tm_V v' then Some empty.[v' <- Tm_V v] else Some empty.[v <- t].
+Definition matching := unifier_help2 true.
+Definition unify := unifier_help2 false.
+
+Lemma compare_var_sym v1 v2: compare_var v1 v2 = compare_var v2 v1.
+Proof. 
+  case: v1 => v1; case: v2 => v2/=; rewrite leq_eqVlt.
+  rewrite eq_sym; case: eqP => //=[->|v21]//; first by rewrite if_same.
+  case: leqP => //=.
+Qed.
+
+Lemma omap_catf0 t: omap [eta catf empty] t = t.
+Proof. by case: t => //=?; rewrite cat0f. Qed.
+
+Lemma omap_catf_refl (t:Sigma): omap [eta catf t] (Some t) = Some t.
+Proof. by rewrite/=; f_equal; apply/fmapP => k; rewrite fnd_cat if_same. Qed.
+
+Lemma unify_V_empty v t: v \notin vars_tm t -> 
+  unify (Tm_V v) t empty = unify_var empty v t.
 Proof.
-  rewrite/unify /vars_nb/= /unify_aux cardfs1/= !deref_empty/=.
-  rewrite/unify_var.
-  case:t => //= v'.
-    rewrite !inE => /eqP H; rewrite !ifF => //; apply/eqP; congruence.
-  move=> t; case: (_ \in _) => //.
+  rewrite/unify/unifier_help1/unifier_help2/unifier_help1 /= !deref_empty/= /unify_var omap_catf0.
+  case:t => //= v'. rewrite !inE eq_sym; case: eqP => //= ?.
+  case: eqP => //; first by congruence.
+  by rewrite compare_var_sym.
 Qed.
 
 Lemma unifier_help_refl h n t s: unifier_help h n t t s = Some s.
 Proof. by elim: n s t => [|n IH] s t//=; case D: deref; rewrite ?eqxx//?IH/=IH//. Qed.
 
-Lemma unify_refl t s: unify t t s = Some s.
-Proof. apply/unifier_help_refl. Qed.
+Lemma unifier_help_refl1 b t s: unifier_help1 b t t s = Some s.
+Proof. by rewrite/unifier_help1 unifier_help_refl omap_catf_refl. Qed.
 
-Lemma unify_help_ground_eq h n t1 t2 s s':
+Lemma unify_refl t s: unify t t s = Some s.
+Proof. apply/unifier_help_refl1. Qed.
+
+(* Lemma unify_help_ground_eq h n t1 t2 s s':
   ground t1 -> ground t2 -> unifier_help h n t1 t2 s = Some s' -> t1 = t2.
 Proof.
   elim: n t1 t2 s s' => //=[|n IH] t1 t2 s s' G1 G2; rewrite !ground_deref//.
@@ -85,22 +107,42 @@ Proof.
   case H1: unifier_help => [sx|]//=.
   case H2: unifier_help => [sy|]//=.
   by move=> [?]; subst; f_equal; apply/IH; eauto.
+Qed. *)
+
+Lemma unify_help_ground h n t1 t2 s: 
+  ground t1 -> ground t2 -> (t1 == t2) = (unifier_help h n t1 t2 s).
+Proof.
+  elim: n t1 t2 s => [|n IH] t1 t2 s/= G1 G2; rewrite !ground_deref//; case: eqP => //.
+  case: t2 G2 => [p|d|v|f a]; case: t1 G1 => [p'|d'|v'|f' a']//; rewrite?(ground_V,ground_app)//.
+  move=> /andP[gf' ga'] /andP[gf ga] H.
+  have:= IH _ _ s gf' gf; case: unifier_help => //s'; case: eqP => //=? _; subst.
+  have:= IH _ _ s' ga' ga; case: unifier_help => //s''; case: eqP => //; congruence.
 Qed.
 
-Lemma unify_help_diff_ground h n t1 t2 s: 
-  ground t1 -> ground t2 -> t1 <> t2 -> unifier_help h n t1 t2 s = None.
+Lemma unify_help_groundx b n t1 t2 s: 
+  ground t1 -> ground t2 -> t1 <> t2 -> unifier_help b n t1 t2 s = None.
 Proof.
-  elim: n t1 t2 s => [|n IH] t1 t2 s/= G1 G2; rewrite !ground_deref//; case: eqP => // _ H.
-  case: t2 G2 H => [p|d|v|f a]; case: t1 G1 => [p'|d'|v'|f' a']; rewrite?(ground_V)//.
-  rewrite !ground_app => /andP[Gf' Ga'] /andP[Gf Ga] H.
-  case X: unifier_help => [s'|]//=.
-  apply: IH => //.
-  have:= unify_help_ground_eq Gf' Gf X; congruence.
+  move=> G1 G2 H; have:= unify_help_ground b n s G1 G2.
+  by case: eqP => //;rewrite/unify; case: unifier_help.
+Qed.
+
+Lemma unify_help1_groundx b t1 t2 s: 
+  ground t1 -> ground t2 -> t1 <> t2 -> unifier_help1 b t1 t2 s = None.
+Proof.
+  move=> G1 G2 H; have:= unify_help_ground b (size_tm t1 + size_tm t2) s G1 G2.
+  rewrite/unifier_help1; case: eqP => // _; case: unifier_help => //.
+Qed.
+
+Lemma unify_help2_groundx b t1 t2 s: 
+  ground t1 -> ground t2 -> t1 <> t2 -> unifier_help2 b t1 t2 s = None.
+Proof.
+  move=> G1 G2 H; have:= unify_help1_groundx b s G1 G2 H.
+  by rewrite/unifier_help2 !ground_deref//.
 Qed.
 
 Lemma unify_diff_ground t1 t2 s: 
   ground t1 -> ground t2 -> t1 <> t2 -> unify t1 t2 s = None.
-Proof. by apply: unify_help_diff_ground. Qed.
+Proof. by apply/unify_help2_groundx. Qed.
 
 Lemma isSomeP T x (P : option T) : P = Some x -> P.
 Proof. by move=> ->. Qed.
@@ -111,35 +153,98 @@ Proof. by move=> ->. Qed.
 Lemma isNoneP1 T (P : option T) : ~~ P -> P = None.
 Proof. case: P => //. Qed.
 
-(*SNIPT: matchunif *)
-Lemma match_unif: 
-  forall t1 t2 s s', matching t1 t2 s = Some s' -> unify t1 t2 s = Some s'.
-(*ENDSNIPT: matchunif *)
+
+Lemma match_help_unif n t1 t2 s s': 
+  unifier_help true n t1 t2 s = Some s' -> unifier_help false n t1 t2 s = Some s'.
 Proof.
-  rewrite/matching/unify/matching_aux/unify_aux => t1 t2.
-  move: (vars_nb _ _) => n.
-  elim: n t1 t2 => [|n IH] t1 t2 s s'/=; first by [].
+  elim: n t1 t2 s s' => [|n IH]//= t1 t2 s s'.
   case D1: deref => [p|d|v|f a];
   case D2: deref => [p'|d'|v'|f' a']//=.
-  case: eqP => //= J.
-  case u1: unifier_help => [sx|]//= u2.
+  case: eqP => // _.
+  case u1: unifier_help => [sy|]//= u2.
   rewrite (IH _ _ _ _ u1)//=.
   by apply: IH.
 Qed.
 
-(*SNIPT: unif_trans *)
-Lemma unif_trans:
-  forall t1 t2 t3 s, unify t1 t2 s -> unify t2 t3 s -> unify t1 t3 s.
-(*ENDSNIPT: unif_trans *)
+Lemma match_unif t1 t2 s s': matching t1 t2 s = Some s' -> unify t1 t2 s = Some s'.
 Proof.
+  rewrite/matching/unify/unifier_help2/unifier_help1.
+  case U1: unifier_help => //=[sx][?]; subst.
+  by rewrite (match_help_unif U1)//.
+Qed.
+
+Lemma ground_vars_card t: ground t -> #|` vars_tm t | = 0.
+Proof.
+  elim: t => //=[v|f Hf a Ha]; rewrite (ground_V, ground_app)//.
+  by move=> /andP[/Hf/cardfs0_eq->]; rewrite fset0U.
+Qed.
+
+Lemma unify_fuel_ground n m b t1 t2 s:
+  ground t1 -> ground t2 ->
+  unifier_help b n t1 t2 s = unifier_help b m t1 t2 s.
+Proof.
+  move=> G1 G2; case: (boolP (t1 == t2)) => /eqP H; subst.
+    by rewrite !unifier_help_refl.
+  by rewrite !unify_help_groundx//.
+Qed.
+
+Lemma unif_fuel n m b t1 t2 s:
+  size_tm (deref s t1) + size_tm (deref s t2) <= n ->
+  size_tm (deref s t1) + size_tm (deref s t2) <= m ->
+  unifier_help b n t1 t2 s = unifier_help b m t1 t2 s.
+Proof.
+  elim: n m t1 t2 s => //=[|n IH] m t1 t2 s Hn Hm.
+    admit.
+  case: m Hm => [|m] Hm//=.
+    admit.
+  case: eqP => // D.
+  case D1: deref => [p|d|v|f a];
+  case D2: deref => [p'|d'|v'|f' a']//=.
+  case: (boolP (ground t1)) => G1.
+    move: D2; rewrite !ground_deref// => ?; subst.
+    move: G1; rewrite !ground_app => /andP[gf' ga'].
+    case: (boolP (ground t2)) => G2.
+      move: D1; rewrite !ground_deref// => ?; subst.
+      move: G2; rewrite !ground_app => /andP[gf ga].
+      rewrite (unify_fuel_ground _ m)//.
+      case: unifier_help => //=s'.
+      rewrite (unify_fuel_ground _ m)//.
+    move: Hn Hm => /=; rewrite deref_App/= addSn !ltnS => Hn Hm.
+    rewrite -(IH m)//=.
+      case U: unifier_help => [sx|]//=.
+      apply: IH.
+
+      admit.
 Admitted.
 
+Require Import Lia.
 
-Lemma unif_ext_sym t1 t2 s s': unify t1 t2 s = Some s' ->
-  exists e, [disjoint domf e & domf s] /\ s' = s + e.
+(*SNIPT: unif_trans *)
+Lemma unif_trans t1 t2 t3 s: unify t1 t2 s -> unify t2 t3 s -> unify t1 t3 s.
+(*ENDSNIPT: unif_trans *)
 Proof.
-  rewrite/unify/unify_aux/vars_nb.
-  move: (_+_)%nat => n; elim: n t1 t2 s s' => //= [|n IH] t1 t2 s s'.
+  (* pose N := (size (vars_tmL t1) + size (vars_tmL t2) + size (vars_tmL t3) + #|` vars_sigma s|)%nat.
+  rewrite/unify -(@unif_fuel N)%nat => //; last first.
+    by rewrite/N/vars_nb leq_add2r -addnA leq_add2l leq_addr.
+  move=> H1.
+  rewrite -(@unif_fuel N)%nat => //; last first.
+    by rewrite/N/vars_nb !leq_add2r leq_addl.
+  move=> H2.
+  rewrite -(@unif_fuel N)%nat => //; last first.
+    by rewrite/N/vars_nb !leq_add2r leq_addr.
+  move: H1 H2.
+  move: @N => /=.
+  remember (_ + _)%nat as n eqn:Hn; elim: n s t1 t2 t3 Hn => [|n IH] s t1 t2 t3 Hn.
+    admit. *)
+Admitted.
+
+Lemma unify_help_ext n t1 t2 s s':
+
+  unifier_help false n t1 t2 s = Some s' ->
+    exists e : finMap lang_V__canonical__choice_Choice Tm,
+      [disjoint domf e & domf s] /\ s' = s + e.
+Proof.
+  elim: n t1 t2 s s' => //= [|n IH] t1 t2 s s'.
     by case: eqP => // H [<-]; exists empty; rewrite catf0 fdisjoint0X.
   case: eqP => // DE; first by move=> [<-]; exists empty; rewrite catf0 fdisjoint0X.
   rewrite/unify_var/=.
@@ -150,13 +255,11 @@ Proof.
   - case D2: deref => [p'|d'|v'|f' a']//= [?]; subst; exists [fmap].[v' <- Tm_D d].
     rewrite catf_setr catf0//= fsetU0 fdisjoint1X; split => //.
     admit.
-  - case: (boolP (_ \in _)) => // vd1[<-]; exists [fmap].[v <- deref s t1].
-    rewrite catf_setr catf0//= fsetU0 fdisjoint1X; split => //.
+  - case: (boolP (_ \in _)) => //.
     admit.
   - case D2: deref => [p|d|v|f' a']//.
       case: (boolP (_ \in _)) => // vd1[<-]; exists [fmap].[v <- Tm_App f a].
       rewrite catf_setr catf0//= fsetU0 fdisjoint1X; split => //.
-
       admit.
     case Uf: unifier_help => [sx|]//= Ua.
     have:= IH _ _ _ _ Uf; have:= IH _ _ _ _ Ua.
@@ -165,20 +268,101 @@ Proof.
     by exists (sz + sy); rewrite catfA domf_cat fdisjointUX R S.
 Admitted.
 
-Lemma unif_sym : forall t1 t2 s, unify t1 t2 s -> unify t2 t1 s.
+
+Lemma unif_ext t1 t2 s s': unify t1 t2 s = Some s' ->
+  exists e, [disjoint domf e & domf s] /\ s' = s + e.
 Proof.
-  rewrite/unify/unify_aux => t1 t2 s; rewrite /vars_nb addnC.
-  move: (_+_)%nat => n; elim: n t1 t2 s => //= [|n IH] t1 t2 s.
+  rewrite/unify/unifier_help2/unifier_help1.
+  case U: unifier_help => [sx|]//=[?]; subst.
+  exists sx; split => //.
+Admitted.
+
+Definition swaps_aux (s : Sigma) :=
+  let d := filterf s (fun x => if s.[?x] is Some (Tm_V v) then true else false) in
+  s.[\ domf d] + [fmap x : codom_vars d => Tm_V (get_father (val x) d)].
+
+Definition swap (sold snew:Sigma) :=
+  (snew.[& domf sold] + swaps_aux snew.[\ domf sold]).
+
+Lemma filter0 (K: choiceType) V f: filterf (@fmap0 K V) f = fmap0.
+Proof. by apply/fmapP => H; rewrite fnd_filterf !not_fnd// if_same. Qed.
+
+Lemma swaps_aux0: swaps_aux fmap0 = fmap0.
+Proof. by apply/fmapP => J; rewrite !not_fnd// /swaps_aux !inE !not_fnd//filter0 codom_vars0. Qed.
+
+Lemma remf_all (K:choiceType) V (s : {fmap K -> V}): s.[\ domf s] = fmap0.
+Proof. apply/fmapP => k; rewrite fnd_rem; case: (boolP (_ \in _)) => ks; rewrite !not_fnd//. Qed.
+
+Lemma swap_refl s: swap s s = s.
+Proof. by rewrite /swap restrictfT remf_all swaps_aux0 catf0. Qed.
+
+Definition is_var t := if t is (Tm_V _) then true else false.
+
+(* Definition principal_unifier sigma A : Prop :=
+ unif sigma A /\ 
+ forall tau, unif tau A -> forall s, tau (sigma s) = tau s. *)
+
+Axiom phi: Tm -> Tm -> Sigma.
+
+Axiom xx: forall t1 t2 s s', 
+  unify t1 t2 s = Some s' -> deref s' t1 = deref s' (deref (phi t1 t2) t1).
+
+(* f X X = f Z Y ====> {X = Z; Z = Y} *)
+(* f Z Y = f X X ====> {Y = X; Z = X} *)
+(* Lemma unif_symP t1 t2 s s':
+  unify t1 t2 s = Some s' -> unify t2 t1 s = Some (swap s s').
+Proof.
+  rewrite/unify/vars_nb addnC.
+  move: (_+_)%nat => n; elim: n t1 t2 s s' => //= [|n IH] t1 t2 s s'.
+    by rewrite/= eq_sym; case: eqP => // D [<-]; rewrite swap_refl.
+  rewrite eq_sym; case: eqP => // DE.
+    by move=> [<-]; rewrite swap_refl.
+  rewrite/unify_var/=; move: DE.
+  case D1: deref => [p|d|v|f a].
+  - case D2: deref => [p'|d'|v'|f' a']//=; move=> DE [<-]; f_equal.
+    admit.
+  - case D2: deref => [p'|d'|v'|f' a']//=; move=> DE [<-]; f_equal.
+    admit.
+  - case: (boolP (_ \in _)) => // H + [<-].
+    case: (boolP (is_var (deref s t1))).
+      case D2: deref => [p'|d'|v'|f' a']//=.
+      rewrite !inE; case: eqP => //?; subst => //.
+      admit.
+    move=> IV Hx.
+    suffices: s.[v <- deref s t1] = (swap s s.[v <- deref s t1]).
+      by move: IV => + <-; case: deref => //.
+    admit.
+  - case D2: deref => [p'|d'|v'|f' a']//=.
+      rewrite !inE; case: (boolP (_ \in _)) => //=vf.
+      case: (boolP (_ \in _)) => //=va _ [<-].
+      admit.
+    move=> H.
+    rewrite-/unify_var.
+    case U1: unifier_help => [sz|]//= U2.
+    have [e[Dx ?]] := unify_help_ext U1; subst.
+    have [e'[Dy ?]] := unify_help_ext U2; subst.
+    have Hf := IH _ _ _ _ U1.
+    have Ha := IH _ _ _ _ U2.
+    rewrite Hf/=.
+Admitted. *)
+
+Lemma unif_sym t1 t2 s: unify t1 t2 s = unify t2 t1 s.
+Proof.
+  rewrite/unify/unifier_help2/unifier_help1.
+  move: (deref _ _) (deref _ _) => {}t1 {}t2.
+  rewrite addnC; move: (_ + _)%nat => n.
+  f_equal.
+  elim: n t1 t2 s => //= [|n IH] t1 t2 s.
     by rewrite/= eq_sym.
   rewrite eq_sym; case: eqP => // DE.
   case D1: deref => [p|d|v|f a]; case D2: deref => [p'|d'|v'|f' a']//=.
-    rewrite/unify_var; case: (boolP (_ \in _)); rewrite//=!inE.
-    rewrite eq_sym; case: eqP => //.
-  case U1: unifier_help => [s'|]//= U2.
-  have := IH _ _ _ (isSomeP U1).
-  case U1': unifier_help => [s''|]//= _.
-  apply: IH.
-Admitted.
+    by rewrite/unify_var !inE eq_sym compare_var_sym.
+  rewrite IH.
+  case U1: unifier_help => [s'|]//=.
+Qed.
+
+(* Lemma unif_sym t1 t2 s: unify t1 t2 s -> unify t2 t1 s.
+Proof. case U: unify => //_; apply/isSomeP. /unif_symP/U. Qed. *)
 
 
 Axiom unif_acyclic: forall t1 t2 s s',
@@ -214,28 +398,13 @@ Qed.
 (*SNIPT: matchdisj *)
 Lemma matching_disj:
   forall s s' t1 t2, vars t1 # domf s -> vars t1 # vars t2 ->
+                                                                  (*SHOULD BE: e `<=` vars (deref s t2)*)
     matching t1 t2 s = Some s' -> exists e, domf s' = domf s `|` e /\ e `<=` vars t2.
 (*ENDSNIPT: matchdisj *)
 Proof.
-  rewrite/matching/matching_aux => s s' t1 t2.
-  move: (vars_nb t1 t2) => n; elim: n t1 t2 s s' => //=[|n IH] t1 t2 s s' H1 H2.
-    by case: eqP =>// D [<-]; exists fset0; rewrite fsetU0 fsub0set//.
-  case: eqP => // D.
-    by move=> [<-]; exists fset0; rewrite fsetU0 fsub0set//.
-  move:D; rewrite (disjoint_deref_refl H1).
-  case D: deref => [p|d|v|f a]; case: t1 H1 H2 D => [p'|d'|v'|f' a']//= H1 H2 D Hx Hy.
-  - move: Hy => [?]; subst; exists [fset v]; rewrite dom_setf fsetUC; split => //.
-    admit.
-  - move: Hy => [?]; subst; exists [fset v]; rewrite dom_setf fsetUC; split => //.
-    admit.
-  - move: Hy; rewrite/unify_var/= inE; case: eqP => H; first by congruence.
-    move=> [?]; subst;exists [fset v]; rewrite dom_setf fsetUC; split => //.
-    admit.
-  - move: Hy; rewrite/unify_var/= inE; case: ifP => // H.
-    move=> [?]; subst;exists [fset v]; rewrite dom_setf fsetUC; split => //.
-    admit.
-  - move: Hy; case U1: unifier_help => //=[sx] U2.
-    have:= IH _ _ _ _ _ _ U1.
+  rewrite/matching/unifier_help2/unifier_help1 => s s' t1 t2.
+  case U: unifier_help => //=[sx] V1 V2[?]; subst.
+  exists (domf sx); rewrite domf_cat; split => //.
 Admitted.
 
 (*SNIPT: matchingmono *)
@@ -268,9 +437,8 @@ Proof.
   have:= match_unif m1.
   have:= match_unif m2.
   move=> H1 H2.
-  apply/unif_sym.
-  apply/unif_trans/isSomeP/H2.
-  apply/unif_sym/isSomeP/H1.
+  rewrite unif_sym in H2.
+  apply/unif_trans/isSomeP/H1/isSomeP/H2.
 Qed.
 
 Axiom matching_V: forall s t d,
